cedar-lean/Cedar/Thm/SymCC/Data/UUF.lean
@@ -26,44 +26,44 @@ open Cedar.SymCC
 
 theorem uuf_attrs_ancs_no_confusion
   {ety₁ ety₂ ancTy} :
-  UUF.attrs_id ety₁ ≠ UUF.ancs_id ety₂ ancTy
+  UUF.attrsId ety₁ ≠ UUF.ancsId ety₂ ancTy
 := by
   apply String.ne_of_data_ne
-  simp [UUF.attrs_id, UUF.ancs_id, toString, String.data]
+  simp [UUF.attrsId, UUF.ancsId, toString, String.data]
 
 theorem uuf_attrs_tag_keys_no_confusion
   {ety₁ ety₂} :
-  UUF.attrs_id ety₁ ≠ UUF.tag_keys_id ety₂
+  UUF.attrsId ety₁ ≠ UUF.tagKeysId ety₂
 := by
   apply String.ne_of_data_ne
-  simp [UUF.attrs_id, UUF.tag_keys_id, toString, String.data]
+  simp [UUF.attrsId, UUF.tagKeysId, toString, String.data]
 
 theorem uuf_attrs_tag_vals_no_confusion
   {ety₁ ety₂} :
-  UUF.attrs_id ety₁ ≠ UUF.tag_vals_id ety₂
+  UUF.attrsId ety₁ ≠ UUF.tagValsId ety₂
 := by
   apply String.ne_of_data_ne
-  simp [UUF.attrs_id, UUF.tag_vals_id, toString, String.data]
+  simp [UUF.attrsId, UUF.tagValsId, toString, String.data]
 
 theorem uuf_tag_vals_tag_keys_no_confusion
   {ety₁ ety₂} :
-  UUF.tag_vals_id ety₁ ≠ UUF.tag_keys_id ety₂
+  UUF.tagValsId ety₁ ≠ UUF.tagKeysId ety₂
 := by
   apply String.ne_of_data_ne
-  simp [UUF.tag_keys_id, UUF.tag_vals_id, toString, String.data]
+  simp [UUF.tagKeysId, UUF.tagValsId, toString, String.data]
 
 theorem uuf_tag_keys_ancs_no_confusion
   {ety₁ ety₂ ancTy} :
-  UUF.tag_keys_id ety₁ ≠ UUF.ancs_id ety₂ ancTy
+  UUF.tagKeysId ety₁ ≠ UUF.ancsId ety₂ ancTy
 := by
   apply String.ne_of_data_ne
-  simp [UUF.tag_keys_id, UUF.ancs_id, toString, String.data]
+  simp [UUF.tagKeysId, UUF.ancsId, toString, String.data]
 
 theorem uuf_tag_vals_ancs_no_confusion
   {ety₁ ety₂ ancTy} :
-  UUF.tag_vals_id ety₁ ≠ UUF.ancs_id ety₂ ancTy
+  UUF.tagValsId ety₁ ≠ UUF.ancsId ety₂ ancTy
 := by
   apply String.ne_of_data_ne
-  simp [UUF.tag_vals_id, UUF.ancs_id, toString, String.data]
+  simp [UUF.tagValsId, UUF.ancsId, toString, String.data]
 
 end Cedar.Thm
